Examples/SECD/LambdaInt.thy
@@ -1,0 +1,289 @@
+theory LambdaInt
+    imports Lambda "../Imp/MemImp" "../../Mergeable/MergeableRAList"
+begin
+
+(* things needed here:
+  - translate calc2 (arith lang) into unified syntax
+  - translate lambda into unified syntax
+  - liftings
+    - challenge (?): using state (S component of SECD) as a memory
+*)
+
+datatype syn =
+  Sl "Lambda.syn"
+  | Sc "calc2" "str" "str"
+  | Si "int"
+  | Cpush
+
+datatype push_syn =
+    Ppush
+  | Pskip
+
+fun lambda_trans :: "syn \<Rightarrow> Lambda.syn" where
+"lambda_trans (Sl l) = l"
+| "lambda_trans _ = Lambda.Sskip"
+
+fun calc_trans :: "syn \<Rightarrow> calc2" where
+"calc_trans (Sc x _ _) = x"
+| "calc_trans _ = Cskip"
+
+fun push_trans :: "syn \<Rightarrow> push_syn" where
+"push_trans Cpush = Ppush"
+| "push_trans _ = Pskip"
+
+fun calc2_key1 :: "syn \<Rightarrow> str  option" where
+"calc2_key1 (Sc _ s1 _) = Some s1"
+| "calc2_key1 _ = None"
+
+fun calc2_key2 :: "syn \<Rightarrow> str  option" where
+"calc2_key2 (Sc _ _ s2) = Some s2"
+| "calc2_key2 _ = None"
+
+(* next, need to lift
+   idea: take key1, key2 out of environment
+   push result onto stack
+*)
+
+type_synonym clos_info = "(childpath * String.literal)"
+
+(* roalist lifting vs oalist lifting? *)
+(* product this with stack 
+   i.e. we need a way to lift onto stack
+  
+*)
+
+(* wrapped versions of SECD state types ('a should already be wrapped) *)
+
+type_synonym 'a envw = "(String.literal, 'a, (childpath * String.literal) swr) roalist"
+
+type_synonym 'a closw = "childpath swr * String.literal swr * 'a envw"
+
+type_synonym 'a secw = "('a + 'a closw) list swr * 'a envw * (childpath * dir) list swr"
+
+type_synonym 'a secdw = "gensyn_skel md_triv option * 'a secw * 'a secw list swr * bool swr"
+
+(* idea: we are pulling the outermost control element to the top level
+   since it is going to be shared with the gensyn evaluator *)
+type_synonym 'a secdw_full = "(childpath) * 'a secdw"
+
+(* idea: secd state + int register for results of int machine *)
+type_synonym state' =
+  "int secd_full * int"
+
+type_synonym state = 
+  "childpath md_triv option * int swr secdw * int swr"
+
+(* starting at state
+- t2 = secdw
+\<rightarrow> t2 = secw
+\<rightarrow> t1 = list swr
+\<rightarrow> list head
+\<rightarrow> inl *)
+
+
+fun push_sem :: "('a :: Bogus) list \<Rightarrow> ('a :: Bogus) list" where
+"push_sem l = bogus#l"
+
+(* full state:
+- secd state
+- int result register
+- some way to push int result onto stack in an idempotent way
+  - one very cheesy way to do this: have a "CPush" instruction that just creates a new
+    list entry using contents of int result register
+*)
+
+(* OK - need to figure out exactly how to do the key lift. It is a little different
+than memimp because the third argument does not live inside the swr we are lifting into.
+*)
+
+(* another lifting for products, needed here:
+   if we can lift each component, we can lift the whole *)
+
+(*
+definition prod_map_pl ::
+  "('x, 'b1, 'c1, 'z2) plifting_scheme \<Rightarrow>
+   ('x, 'b2, 'c2, 'z3) plifting_scheme \<Rightarrow>
+   ('x, 'a, 'b1 * 'b2, 'z1) plifting_scheme \<Rightarrow>
+   ('x, 'a, 'c1 * 'c2) plifting" where
+"prod_map_pl lfst lsnd l =
+  \<lparr> LUpd =
+    (\<lambda> s a b . (case a of (a1, a2) \<Rightarrow>
+                  (case b of (b1, b2) \<Rightarrow>
+                    (LUpd t1 s a1 b1, LUpd t2 s a2 b2))))
+  , LOut =
+    (\<lambda> s b . (case b of (b1, b2) \<Rightarrow>
+                (LOut t1 s b1, LOut t2 s b2)))
+  , LBase =
+    (\<lambda> s . (LBase t1 s, LBase t2 s)) \<rparr>"
+
+definition prod_l ::
+  "('x, 'a1, 'b1, 'z1) lifting_scheme \<Rightarrow>
+   ('x, 'a2, 'b2, 'z2) lifting_scheme \<Rightarrow>
+   ('x, 'a1 * 'a2, 'b1 * 'b2) lifting" where
+"prod_l t1 t2 =
+  plifting.extend (prod_pl t1 t2)
+    \<lparr> LPost = (\<lambda> s b . (case b of (b1, b2) \<Rightarrow> (LPost t1 s b1, LPost t2 s b2))) \<rparr>"
+*)
+
+term "snd_l (snd_l (fst_l (snd_l ( (roalist_l calc2_key1 ((prio_l_keep o option_l o triv_l) id_l))))))"
+
+term "(prod_l (
+    merge_l
+      (roalist_l calc2_key1 ((prio_l_keep o option_l o triv_l) id_l))
+      (roalist_l calc2_key2 ((prio_l_keep o option_l o triv_l) id_l)))
+        ((prio_l_inc o option_l o triv_l) id_l))"
+
+definition calc2_key_lift :: "(syn, calc2_state, int swr envw * int swr) lifting" where
+"calc2_key_lift =
+  prod_deassoca_l (prod_l (
+    merge_l
+      (roalist_l calc2_key1 ((prio_l_keep o option_l o triv_l) id_l))
+      (roalist_l calc2_key2 ((prio_l_keep o option_l o triv_l) id_l)))
+        ((prio_l_inc o option_l o triv_l) id_l))"
+
+(*
+term "((snd_l o snd_l o fst_l o fst_l o prio_l_inc o option_l o triv_l o list_hd_l o inl_l ) 
+        (roalist_l calc2_key1 ((prio_l_keep o option_l o triv_l) id_l)))"
+
+term "((snd_l o snd_l o fst_l o snd_l o prio_l_inc o option_l o triv_l o list_hd_l o inl_l ) 
+        (roalist_l calc2_key1 ((prio_l_keep o option_l o triv_l) id_l))) :: (syn, calc2_state, state) lifting"
+
+*)
+
+definition calc2_lift :: "(syn, calc2_state, state) lifting" where
+"calc2_lift =
+merge_l
+  ((t2_l o t2_l o t2_l) (roalist_l calc2_key1 ((prio_l_inc o option_l o triv_l) id_l)))
+  (merge_l
+    ((t2_l o t2_l o t2_l) (roalist_l calc2_key1 ((prio_l_inc o option_l o triv_l) id_l)))
+    ((t2_l o t2_l o t1_l o prio_l_inc o option_l o triv_l o list_hd_l o inl_l)
+      ((prio_l_inc o option_l o triv_l) id_l)))"
+
+(* scratch work for building up calc2_lift *)
+
+term "((t2_l o t2_l o t2_l ) 
+        (roalist_l calc2_key1 ((prio_l_inc o option_l o triv_l) id_l)))"
+
+term "merge_l
+      ((t2_l o t2_l o t2_l ) 
+        (roalist_l calc2_key1 ((prio_l_inc o option_l o triv_l) id_l)))
+       ((t2_l o t2_l o t2_l ) 
+        (roalist_l calc2_key1 ((prio_l_inc o option_l o triv_l) id_l))) :: (syn, int * int, state) lifting"
+
+term "(t2_l o t2_l o t1_l o prio_l_inc o option_l o triv_l o list_hd_l o inl_l)
+      ((prio_l_inc o option_l o triv_l) id_l) :: (syn, int, state) lifting"
+
+term "
+merge_l
+  ((t2_l o t2_l o t2_l) (roalist_l calc2_key1 ((prio_l_inc o option_l o triv_l) id_l)))
+  (merge_l
+    ((t2_l o t2_l o t2_l) (roalist_l calc2_key1 ((prio_l_inc o option_l o triv_l) id_l)))
+    ((t2_l o t2_l o t1_l o prio_l_inc o option_l o triv_l o list_hd_l o inl_l)
+      ((prio_l_inc o option_l o triv_l) id_l)))
+:: (syn, calc2_state, state) lifting
+"
+
+definition calc_sem_l :: "syn \<Rightarrow> state \<Rightarrow> state" where
+"calc_sem_l =
+  l_map_s id
+  calc2_lift
+  (calc2_sem o calc_trans)"
+
+term "prod_l "
+
+(* OK, so it looks like we need map-liftings for
+- sum
+- roalist
+both are done now
+*)
+(* secd_full has:
+   - childpath \<Rightarrow> lift into state
+   - secd \<Rightarrow> lift into secd_w
+   - int (unneeded, use fst/deassoc.) *)
+
+definition env_lift ::
+"(syn, ('a :: Bogus) env, 'a swr envw) lifting"
+where
+"env_lift =
+  roalist_map_l ((prio_l_inc o ot_l) id_l) 
+                ((prio_l_inc o ot_l) id_l)"
+
+definition clos_lift ::
+"(syn, ('a :: Bogus) clos, 'a swr closw) lifting" where
+"clos_lift =
+  prod_l
+    ((prio_l_inc o ot_l) id_l)
+    (prod_l
+      ((prio_l_inc o ot_l) id_l)
+      (env_lift))"
+
+definition sec_lift ::
+"(syn, ('a :: Bogus) sec, 'a swr secw) lifting" where
+"sec_lift =
+  prod_l
+    ((prio_l_inc o ot_l o list_map_l)
+      (sum_map_l 
+        ((prio_l_inc o ot_l) id_l)
+        clos_lift))
+  (prod_l
+      env_lift
+      ((prio_l_inc o ot_l) id_l))"
+
+definition secd_lift ::
+"(syn, ('a :: Bogus) secd, 'a swr secdw) lifting" where
+"secd_lift =
+  prod_l
+    (ot_l id_l)
+    (prod_l
+      sec_lift
+      (prod_l
+        ((prio_l_inc o ot_l) (list_map_l sec_lift))
+        ((prio_l_inc o ot_l) id_l)))"
+
+
+definition lambda_state_lift ::
+"(syn, (int) secd_full,  state) lifting"
+where
+"lambda_state_lift =
+  prod_l
+    (ot_l id_l)
+    (fst_l secd_lift)"
+
+definition lambda_sem_l :: "syn \<Rightarrow> state \<Rightarrow> state" where
+"lambda_sem_l =
+  l_map_s id
+    lambda_state_lift
+    (secd_sem o lambda_trans)"
+
+definition sems where
+"sems = [calc_sem_l, lambda_sem_l]"
+
+definition gsx_info :: 
+  "syn \<Rightarrow> state \<Rightarrow> (gensyn_skel * unit gs_result)" where
+"gsx_info syn st =
+  secd_gsx_info
+    (lambda_trans syn)
+    (LOut lambda_state_lift syn st)"
+
+definition sem_final :: "(syn, state) x_sem'" where
+"sem_final =
+  l_map_s id
+    (prod_fan_l gsx_info id_l) (pcomps sems)"
+
+definition gsx :: "syn gensyn \<Rightarrow> childpath \<Rightarrow> state \<Rightarrow> nat \<Rightarrow> state option" where
+"gsx = gensyn_sem_exec (xsem sem_final)"
+
+(* next: testprog, initial states, etc. *)
+
+
+(* now we need to figure out how to push
+the wrapping through the list. *)
+(*
+term "
+prod_l
+  (triv_l ((t2_l
+*)
+
+(* then we just need to give liftings for plugging everything together. *)
+
+end
